get BlockCache compiling

disk-betree/BlockCache.dfy
@@ -1,61 +1,95 @@
 include "DiskBetree.dfy"
+include "../lib/sequences.dfy"
+include "../lib/Maps.dfy"
 
 module BlockCache {
+  import opened Sequences
+  import opened Maps
+
   datatype Constants = Constants()
 
-  // psssst T = Node but dodn't tell anybody
+  // psssst Node = DiskBetree.Node but dodn't tell anybody
   import DiskBetree
-  type T<Value> = DiskBetree.Node<Value>
-  function Successor(node: T): iset<Reference> { node.children.Values }
+  type Node<Value> = DiskBetree.Node<Value>
+  function Successors(node: Node): iset<Reference> { node.children.Values }
+
+  import BlockInterface
+  type Reference = BlockInterface.Reference
 
   // Stuff for communicating with Disk (probably move to another file?)
+
+  type LBA
+
+  function SuperblockLBA(k: Constants) : LBA
 
   datatype Superblock = Superblock(
       lbas: map<Reference, LBA>,
       refcounts: map<Reference, int>)
 
-  datatype Sector =
-    | SectorBlock(block: T)
-    | SectorSuperblock(superblock)
+  datatype Sector<Value> =
+    | SectorBlock(block: Node<Value>)
+    | SectorSuperblock(superblock: Superblock)
 
   // TODO make async
-  datatype DiskOp =
-    | Write(lba: LBA, sector: Sector)
-    | Read(lba: LBA, sector: Sector)
+  datatype DiskOp<Value> =
+    | Write(lba: LBA, sector: Sector<Value>)
+    | Read(lba: LBA, sector: Sector<Value>)
     | NoDiskOp
 
   // BlockCache stuff
 
-  datatype CacheLine<T> = CacheLine(block: T)
+  datatype CacheLine<Value> = CacheLine(block: Node<Value>)
 
-  datatype Variables =
+  datatype Variables<Value> =
     | Ready(
-        persistentSuperblock: SuperBlock,
-        ephemeralSuperblock: SuperBlock,
-        cache: map<Reference, CacheLine>)
+        persistentSuperblock: Superblock,
+        ephemeralSuperblock: Superblock,
+        cache: map<Reference, CacheLine<Value>>)
     | Unready
 
-  predicate IsNotDirty(s: Variables, ref: Reference) {
+  predicate IsNotDirty(s: Variables, ref: Reference)
+  requires s.Ready?
+  {
     ref in s.ephemeralSuperblock.lbas
   }
-  predicate IsAllocated(s: Variables, ref: Reference) {
+  predicate IsAllocated(s: Variables, ref: Reference)
+  requires s.Ready?
+  {
     ref in s.ephemeralSuperblock.refcounts
   }
 
-  datatype Step =
+  datatype Step<Value> =
     | WriteBackStep(ref: Reference)
     | WriteBackSuperblockStep
-    | DirtyStep(ref: Reference, block: T)
-    | Alloc(ref: Reference, block: T)
+    | DirtyStep(ref: Reference, block: Node<Value>)
+    | Alloc(ref: Reference, block: Node<Value>)
     | Unalloc(ref: Reference)
     | PageInStep(ref: Reference)
     | PageInSuperblockStep
     | EvictStep(ref: Reference)
     // TODO page in superblock
 
-  predicate refCountsChangeConsistently(s: Variables, s': Variables, ref: Reference)
+  predicate refCountsChangeConsistently(
+      refcounts: map<Reference, int>,
+      refcounts': map<Reference, int>,
+      cache: map<Reference, CacheLine>,
+      cache': map<Reference, CacheLine>,
+      ref: Reference)
   {
-    forall 
+    && (forall r :: r in refcounts && r != ref ==> (
+      MapsTo(refcounts', r,
+          refcounts[r] +
+          (if ref in cache' && r in Successors(cache'[ref].block) then 1 else 0) -
+          (if ref in cache && r in Successors(cache[ref].block) then 1 else 0)
+      )
+    ))
+    && (ref in refcounts && ref in refcounts' ==>
+      MapsTo(refcounts', ref,
+          refcounts[ref] +
+          (if ref in cache' && ref in Successors(cache'[ref].block) then 1 else 0) -
+          (if ref in cache && ref in Successors(cache[ref].block) then 1 else 0)
+      )
+    )
   }
 
   predicate WriteBack(k: Constants, s: Variables, s': Variables, dop: DiskOp, ref: Reference)
@@ -63,9 +97,9 @@ module BlockCache {
     && s.Ready?
     && dop.Write?
     && ref in s.cache
-    && dop.lba !in persistentSuperblock.lbas.Values
-    && dop.lba !in ephemeralSuperblock.lbas.Values
-    && dop.sector == SectorBlock(s.cache[dop.lba].block)
+    && dop.lba !in s.persistentSuperblock.lbas.Values
+    && dop.lba !in s.ephemeralSuperblock.lbas.Values
+    && dop.sector == SectorBlock(s.cache[ref].block)
     && s'.Ready?
     && s'.persistentSuperblock == s.persistentSuperblock
     && s'.ephemeralSuperblock.lbas == s.ephemeralSuperblock.lbas[ref := dop.lba]
@@ -80,106 +114,111 @@ module BlockCache {
     && dop.lba == SuperblockLBA(k)
     && dop.sector == SectorSuperblock(s.ephemeralSuperblock)
     && s.cache.Keys <= s.ephemeralSuperblock.lbas.Keys
-    && s' == s[persistentSuperblock := s.ephemeralSuperblock]
+    && s' == s.(persistentSuperblock := s.ephemeralSuperblock)
   }
 
-  predicate Dirty(k: Constants, s: Variables, s': Variables, dop: DiskOp, ref: Reference, block: T)
+  predicate Dirty(k: Constants, s: Variables, s': Variables, dop: DiskOp, ref: Reference, block: Node)
   {
     // Possibly allocs ref, possibly overwrites it.
     && s.Ready?
-    && dop.NoDiskOp
+    && dop.NoDiskOp?
     && ref in s.cache
     && s'.Ready?
     && s'.cache == s.cache[ref := CacheLine(block)]
-    && s'.persistentSuperblock == s.persistenSuperblock
+    && s'.persistentSuperblock == s.persistentSuperblock
 
-    && s'.ephemeralSuperblock.lbas == s.ephemeralSuperblock.lbas[ref := null]
+    && s'.ephemeralSuperblock.lbas == MapRemove(s.ephemeralSuperblock.lbas, {ref})
 
-    && refCountsChangeConsistently(s.ephemeralSuperblock.refcounts, s'.ephemeralSuperblock.refcounts, s.cache, ref)
+    && refCountsChangeConsistently(s.ephemeralSuperblock.refcounts, s'.ephemeralSuperblock.refcounts, s.cache, s'.cache, ref)
   }
 
-  predicate Alloc(k: Constants, s: Variables, s': Variables, dop: DiskOp, ref: Reference, block: T)
+  predicate Alloc(k: Constants, s: Variables, s': Variables, dop: DiskOp, ref: Reference, block: Node)
   {
     // Possibly allocs ref, possibly overwrites it.
     && s.Ready?
-    && dop.NoDiskOp
+    && dop.NoDiskOp?
     && ref !in s.cache
     && !IsAllocated(s, ref)
     && s'.Ready?
     && s'.cache == s.cache[ref := CacheLine(block)]
-    && s'.persistentSuperblock == s.persistenSuperblock
+    && s'.persistentSuperblock == s.persistentSuperblock
 
     && s'.ephemeralSuperblock.lbas == s.ephemeralSuperblock.lbas
 
-    && refCountsChangeConsistently(s.ephemeralSuperblock.refcounts, s'.ephemeralSuperblock.refcounts, s.cache, ref)
-    && s'.ephemeralSuperblock.refcounts[ref] == 0
+    && refCountsChangeConsistently(s.ephemeralSuperblock.refcounts, s'.ephemeralSuperblock.refcounts, s.cache, s'.cache, ref)
+    && MapsTo(s'.ephemeralSuperblock.refcounts, ref, 0)
   }
 
   predicate Unalloc(k: Constants, s: Variables, s': Variables, dop: DiskOp, ref: Reference)
   {
     && s.Ready?
-    && dop.NoDiskOp
-    && IsAllocated(s, ref)
+    && dop.NoDiskOp?
+
+    // This kind of sucks. It needs to be in cache so we know it's successors we can decrement
+    // refcounts. TODO There is an optimization to be made such that we can unalloc leaves
+    // which are not in cache (becasue they have no outgoing pointers)
+    && ref in s.cache 
+
     && s'.Ready?
     && s'.persistentSuperblock == s.persistentSuperblock
-    && s'.ephemeralSuperblock.lbas == RemoveFromMap(s.ephemeralSuperblock.lbas, ref)
-    && s'.cache == RemoveFromMap(s.cache, ref)
-    && refCountsChangeConsistently(s.ephemeralSuperblock.refcounts, s'.ephemeralSuperblock.refcounts, s.cache, ref)
+    && s'.ephemeralSuperblock.lbas == MapRemove(s.ephemeralSuperblock.lbas, {ref})
+    && s'.cache == MapRemove(s.cache, {ref})
+    && refCountsChangeConsistently(s.ephemeralSuperblock.refcounts, s'.ephemeralSuperblock.refcounts, s.cache, s'.cache, ref)
     && ref !in s'.ephemeralSuperblock.refcounts
   }
 
   predicate PageIn(k: Constants, s: Variables, s': Variables, dop: DiskOp, ref: Reference)
   {
     && s.Ready?
-    && dop.Read
+    && dop.Read?
     && IsAllocated(s, ref)
     && IsNotDirty(s, ref)
-    && s.ephemeralSuperblock[ref].lba == dop.lba
+    && s.ephemeralSuperblock.lbas[ref] == dop.lba
     && dop.sector.SectorBlock?
-    && s' == s[cache := s.cache[ref := CacheLine(dop.sector.block)]]
+    && s' == s.(cache := s.cache[ref := CacheLine(dop.sector.block)])
   }
 
   predicate PageInSuperblock(k: Constants, s: Variables, s': Variables, dop: DiskOp, ref: Reference)
   {
     && s.Unready?
-    && dop.Read
-    && dop.lba == SuperblockLBA
-    && dop.sector.superblock?
+    && dop.Read?
+    && dop.lba == SuperblockLBA(k)
+    && dop.sector.SectorSuperblock?
     && s' == Ready(dop.sector.superblock, dop.sector.superblock, map[])
   }
 
   predicate Evict(k: Constants, s: Variables, s': Variables, dop: DiskOp, ref: Reference)
   {
     && s.Ready?
-    && dop.NoDiskOp
+    && dop.NoDiskOp?
     && ref in s.cache
     && IsNotDirty(s, ref)
-    && s' == s[cache := RemoveFromMap(s.cache, ref)]
+    && s' == s.(cache := MapRemove(s.cache, {ref}))
   }
 
-  predicate WFSuperblock(superblock: Superblock)
+  predicate WFSuperblock(k: Constants, superblock: Superblock)
   {
-    && SuperBlockLBA !in superblock.lbas.Values
+    && SuperblockLBA(k) !in superblock.lbas.Values
     && superblock.lbas.Keys <= superblock.refcounts.Keys
   }
 
   predicate Init(k: Constants, s: Variables)
   {
-    s == Unready(map[])
+    s == Unready
   }
 
   predicate Inv(k: Constants, s: Variables)
   {
     match s {
-      case Ready(persistentSuperblock, ephemeralSuperblock, cache) => {
-        && WFSuperblock(s.persistentSuperblock)
-        && WFSuperblock(s.ephemeralSuperblock)
+      case Ready(persistentSuperblock, ephemeralSuperblock, cache) => (
+        && WFSuperblock(k, s.persistentSuperblock)
+        && WFSuperblock(k, s.ephemeralSuperblock)
         && s.persistentSuperblock.lbas.Keys == s.persistentSuperblock.refcounts.Keys
-        && s.cache.Keys <= s.ephemeralSuperblock.refcounts
-      }
-      case Unready(cache) => {
+        && s.cache.Keys <= s.ephemeralSuperblock.refcounts.Keys
+      )
+      case Unready => (
         true
-      }
+      )
     }
   }
 }
